Mincost_Flow_Algorithms/Use_Orlins_Algorithm/Usage_Multigraph.thy
@@ -87,7 +87,7 @@ value edges
 value G
 value "dfs_initial_state (1::nat)"   
 value "dfs_impl G 9 (dfs_initial_state 0)"
-value "vset_diff (nbs 1) (nbs 2)"
+value "vset_diff (nbs edges (1::nat)) (nbs edges (2::nat))"
 end
 
 context begin
